CoqOfRust/core/fmt.v
@@ -1,0 +1,302 @@
+Require Import CoqOfRust.lib.lib.
+Require CoqOfRust.core.result.
+
+(* 
+pub enum Alignment {
+  Left,
+  Right,
+  Center,
+}
+*)
+Module Alignment.
+  Inductive t : Set := 
+  | Left
+  | Right
+  | Center
+  .
+End Alignment.
+Definition Alignment : Set := Alignment.t.
+
+Parameter Error : Set.
+
+Definition Result : Set := result.Result unit Error.
+
+Module Arguments.
+  Parameter t : Set.
+End Arguments.
+Definition Arguments := Arguments.t.
+
+Module Write.
+  Class Trait (Self : Set) : Set := {
+    write_str `{State.Trait} : mut_ref Self -> ref str -> M Result;
+    write_char `{State.Trait} : mut_ref Self -> char -> M Result;
+    write_fmt `{State.Trait} : mut_ref Self -> Arguments -> M Result;
+  }.
+
+  Global Instance Method_write_str `{State.Trait} `(Trait) : Notation.Dot "write_str" := {
+    Notation.dot := write_str;
+  }.
+  Global Instance Method_write_char `{State.Trait} `(Trait) : Notation.Dot "write_char" := {
+    Notation.dot := write_char;
+  }.
+  Global Instance Method_write_fmt `{State.Trait} `(Trait) : Notation.Dot "write_fmt" := {
+    Notation.dot := write_fmt;
+  }.
+End Write.
+
+Module Formatter.
+  Parameter t : Set.
+End Formatter.
+Definition Formatter := Formatter.t.
+
+Module DebugTuple.
+  Parameter t : Set.
+End DebugTuple.
+Definition DebugTuple := DebugTuple.t.
+
+Module Display.
+  Class Trait (Self : Set) : Set := {
+    fmt `{State.Trait} : ref Self -> mut_ref Formatter -> M Result;
+  }.
+End Display.
+
+Module Debug.
+  Class Trait (Self : Set) : Set := {
+    fmt `{State.Trait} : ref Self -> mut_ref Formatter -> M Result;
+  }.
+End Debug.
+
+Module ImplDebugTuple.
+  Definition Self := DebugTuple.
+
+  (** field(&mut self, value: &dyn Debug) -> &mut DebugTuple<'a, 'b> *)
+  Parameter field :
+    forall `{State.Trait} {T : Set} `{Debug.Trait T},
+      mut_ref Self -> ref T -> M (mut_ref DebugTuple).
+
+  Global Instance Method_field `{State.Trait} {T : Set} `{Debug.Trait T} :
+    Notation.Dot "field" := {
+    Notation.dot := field;
+  }.
+
+  (** finish(&mut self) -> Result<(), Error> *)
+  Parameter finish : forall `{State.Trait}, mut_ref Self -> M Result.
+
+  Global Instance Method_finish `{State.Trait} :
+    Notation.Dot "finish" := {
+    Notation.dot := finish;
+  }.
+End ImplDebugTuple.
+
+Module ImplFormatter.
+  Definition Self := Formatter.
+
+  Parameter new : forall `{State.Trait} {W : Set} `{Write.Trait W},
+    mut_ref W -> M Formatter.
+
+  Global Instance Formatter_new `{State.Trait} {W : Set} `{Write.Trait W} :
+    Notation.DoubleColon Formatter "new" := {
+    Notation.double_colon := new;
+  }.
+
+  (*
+  pub(super) fn debug_tuple_new<'a, 'b>(
+      fmt: &'a mut fmt::Formatter<'b>,
+      name: &str,
+  ) -> DebugTuple<'a, 'b> {
+      let result = fmt.write_str(name);
+      DebugTuple { fmt, result, fields: 0, empty_name: name.is_empty() }
+  }
+  *)
+  Parameter debug_tuple_new :
+    forall `{State.Trait} (fmt : mut_ref Formatter) (name : ref str),
+      M DebugTuple.
+
+  Global Instance Method_debug_tuple `{State.Trait} :
+    Notation.Dot "debug_tuple_new" := {
+    Notation.dot := debug_tuple_new;
+  }.
+
+  (*
+  pub fn debug_tuple_field1_finish<'b>(&'b mut self, name: &str, value1: &dyn Debug) -> Result {
+      let mut builder = builders::debug_tuple_new(self, name);
+      builder.field(value1);
+      builder.finish()
+  }
+  *)
+  Definition debug_tuple_field1_finish `{State.Trait} {T : Set}
+    `{core.fmt.Debug.Trait T} (f : core.fmt.Formatter) (x : ref str) (y : T) :
+    M core.fmt.Result :=
+    let* dt := f.["debug_tuple_new"] x in
+    let* fld := dt.["field"] y in
+    fld.["finish"].
+
+  Global Instance Formatter_debug_tuple_field1_finish `{State.Trait}
+    {T : Set} `{core.fmt.Debug.Trait T} :
+    Notation.DoubleColon core.fmt.Formatter "debug_tuple_field1_finish" := {
+    Notation.double_colon := debug_tuple_field1_finish (T := T);
+  }.
+End ImplFormatter.
+
+Module Octal.
+  Class Trait (Self : Set) : Set := {
+    fmt `{State.Trait} : ref Self -> mut_ref Formatter -> M Result;
+  }.
+End Octal.
+
+Module LowerHex.
+  Class Trait (Self : Set) : Set := {
+    fmt `{State.Trait} : ref Self -> mut_ref Formatter -> M Result;
+  }.
+End LowerHex.
+
+Module UpperHex.
+  Class Trait (Self : Set) : Set := {
+    fmt `{State.Trait} : ref Self -> mut_ref Formatter -> M Result;
+  }.
+End UpperHex.
+
+Module Pointer.
+  Class Trait (Self : Set) : Set := {
+    fmt `{State.Trait} : ref Self -> mut_ref Formatter -> M Result;
+  }.
+End Pointer.
+
+Module Binary.
+  Class Trait (Self : Set) : Set := {
+    fmt `{State.Trait} : ref Self -> mut_ref Formatter -> M Result;
+  }.
+End Binary.
+
+Module LowerExp.
+  Class Trait (Self : Set) : Set := {
+    fmt `{State.Trait} : ref Self -> mut_ref Formatter -> M Result;
+  }.
+End LowerExp.
+
+Module UpperExp.
+  Class Trait (Self : Set) : Set := {
+    fmt `{State.Trait} : ref Self -> mut_ref Formatter -> M Result;
+  }.
+End UpperExp.
+
+Module ArgumentV1.
+  Parameter t : Set.
+End ArgumentV1.
+Definition ArgumentV1 := ArgumentV1.t.
+
+Module ImplArgumentV1.
+  Definition Self := ArgumentV1.
+
+  Parameter new :
+    forall `{State.Trait} {T : Set},
+    ref T -> (ref T -> mut_ref Formatter -> M Result) -> M Self.
+
+  Global Instance ArgumentV1_new `{State.Trait} {T : Set} :
+    Notation.DoubleColon ArgumentV1 "new" := {
+    Notation.double_colon := new (T := T);
+  }.
+
+  Parameter new_display :
+    forall `{State.Trait} {T : Set} `{Display.Trait T}, ref T -> M Self.
+
+  Global Instance ArgumentV1_new_display
+    `{State.Trait} {T : Set} `{Display.Trait T} :
+    Notation.DoubleColon ArgumentV1 "new_display" := {
+    Notation.double_colon := new_display (T := T);
+  }.
+
+  Parameter new_debug :
+    forall `{State.Trait} {T : Set} `{Debug.Trait T}, ref T -> M Self.
+
+  Global Instance ArgumentV1_new_debug
+    `{State.Trait} {T : Set} `{Debug.Trait T} :
+    Notation.DoubleColon ArgumentV1 "new_debug" := {
+    Notation.double_colon := new_debug (T := T);
+  }.
+
+  Parameter new_octal :
+    forall `{State.Trait} {T : Set} `{Octal.Trait T}, ref T -> M Self.
+
+  Global Instance ArgumentV1_new_octal
+    `{State.Trait} {T : Set} `{Octal.Trait T} :
+    Notation.DoubleColon ArgumentV1 "new_octal" := {
+    Notation.double_colon := new_octal (T := T);
+  }.
+
+  Parameter new_lower_hex :
+    forall `{State.Trait} {T : Set} `{LowerHex.Trait T}, ref T -> M Self.
+
+  Global Instance ArgumentV1_new_lower_hex
+    `{State.Trait} {T : Set} `{LowerHex.Trait T} :
+    Notation.DoubleColon ArgumentV1 "new_lower_hex" := {
+    Notation.double_colon := new_lower_hex (T := T);
+  }.
+
+  Parameter new_upper_hex :
+    forall `{State.Trait} {T : Set} `{UpperHex.Trait T}, ref T -> M Self.
+
+  Global Instance ArgumentV1_new_upper_hex
+    `{State.Trait} {T : Set} `{UpperHex.Trait T} :
+    Notation.DoubleColon ArgumentV1 "new_upper_hex" := {
+    Notation.double_colon := new_upper_hex (T := T);
+  }.
+
+  Parameter new_pointer :
+    forall `{State.Trait} {T : Set} `{Pointer.Trait T}, ref T -> M Self.
+
+  Global Instance ArgumentV1_new_pointer
+    `{State.Trait} {T : Set} `{Pointer.Trait T} :
+    Notation.DoubleColon ArgumentV1 "new_pointer" := {
+    Notation.double_colon := new_pointer (T := T);
+  }.
+
+  Parameter new_binary :
+    forall `{State.Trait} {T : Set} `{Binary.Trait T}, ref T -> M Self.
+
+  Global Instance ArgumentV1_new_binary
+    `{State.Trait} {T : Set} `{Binary.Trait T} :
+    Notation.DoubleColon ArgumentV1 "new_binary" := {
+    Notation.double_colon := new_binary (T := T);
+  }.
+
+  Parameter new_lower_exp :
+    forall `{State.Trait} {T : Set} `{LowerExp.Trait T}, ref T -> M Self.
+
+  Global Instance ArgumentV1_new_lower_exp
+    `{State.Trait} {T : Set} `{LowerExp.Trait T} :
+    Notation.DoubleColon ArgumentV1 "new_lower_exp" := {
+    Notation.double_colon := new_lower_exp (T := T);
+  }.
+
+  Parameter new_upper_exp :
+    forall `{State.Trait} {T : Set} `{UpperExp.Trait T}, ref T -> M Self.
+
+  Global Instance ArgumentV1_new_upper_exp
+    `{State.Trait} {T : Set} `{UpperExp.Trait T} :
+    Notation.DoubleColon ArgumentV1 "new_upper_exp" := {
+    Notation.double_colon := new_upper_exp (T := T);
+  }.
+End ImplArgumentV1.
+
+Module ImplArguments.
+  Parameter new_const :
+    forall `{State.Trait}, ref (list (ref str)) -> M Arguments.
+
+  Global Instance Arguments_new_const `{State.Trait} :
+    Notation.DoubleColon Arguments "new_const" := {
+    Notation.double_colon := new_const;
+  }.
+
+  Parameter new_v1 :
+    forall `{State.Trait},
+      ref (list (ref str)) -> ref (list ArgumentV1) -> M Arguments.
+
+  Global Instance Arguments_new_v1 `{State.Trait} :
+    Notation.DoubleColon Arguments "new_v1" := {
+    Notation.double_colon := new_v1;
+  }.
+End ImplArguments.
+
+Global Instance Write_for_Formatter : Write.Trait Formatter.
+Admitted.
